added expunge to framework

Isabelle/IMAP.thy
@@ -23,17 +23,16 @@ abbreviation filesystem ::
 where
   "filesystem I \<equiv> snd I"
 
-
 definition validState ::
   "('a, 'b) imap \<Rightarrow> bool"
 where
   "validState I = ((\<forall> (a, _) \<in> folderset I . (filesystem I) a \<noteq> None)
   \<and> (\<forall> f . (filesystem I) f \<noteq> None \<longrightarrow> (\<exists> (a, _) \<in> folderset I . a = f)))"
 
-definition Msg ::
+definition msgReplace ::
   "'b \<Rightarrow> 'b \<Rightarrow> 'b set \<Rightarrow> 'b set"
 where
-  "Msg msgold msgnew S = (S - {msgold}) \<union> {msgnew}"
+  "msgReplace msgold msgnew S = (S - {msgold}) \<union> {msgnew}"
 
 definition msgLookup ::
   "'a \<Rightarrow> 'b \<Rightarrow> ('a, 'b) imap \<Rightarrow> bool"
@@ -83,7 +82,6 @@ where
       Some msgset \<Rightarrow> (filesystem I)(f := Some (msgset \<union> {m}))
   ))"
 
-
 definition store_pre ::
   "'a \<Rightarrow> 'b \<Rightarrow> 'b \<Rightarrow> ('a, 'b) imap \<Rightarrow> bool"
 where
@@ -96,18 +94,18 @@ where
   (folderset I,
   (case (filesystem I)(f) of
       None \<Rightarrow> filesystem I |
-      Some msgset \<Rightarrow> (filesystem I)(f := Some (Msg msgold msgnew msgset))
+      Some msgset \<Rightarrow> (filesystem I)(f := Some (msgReplace msgold msgnew msgset))
   ))"
 
-definition EXPUNGE_atSource ::
+definition expunge_pre ::
   "'a \<Rightarrow> 'b \<Rightarrow> ('a, 'b) imap \<Rightarrow> bool"
 where
-  "EXPUNGE_atSource f m I = ((\<exists> (a, _) \<in> folderset I . a = f) \<and> msgLookup f m I)"
+  "expunge_pre f m I = ((\<exists> (a, _) \<in> folderset I . a = f) \<and> msgLookup f m I)"
 
-definition EXPUNGE_downstream ::
+definition expunge ::
   "'a \<Rightarrow> 'b \<Rightarrow> ('a, 'b) imap \<Rightarrow> ('a, 'b) imap"
 where
-  "EXPUNGE_downstream f m I =
+  "expunge f m I =
   (folderset I,
   (case (filesystem I)(f) of
       None \<Rightarrow> filesystem I |
@@ -225,12 +223,10 @@ assumes
 shows "validState (create e n I)"
 proof -
   show ?thesis
-  using validS
-  unfolding create_def add_def validState_def create_pre_def
-  apply simp
-  by (simp add: split_def)
+    using validS
+    unfolding create_def add_def validState_def create_pre_def
+    by (simp add: split_def)
 qed
-
 
 lemma delete_valid:
 fixes
@@ -243,26 +239,25 @@ assumes
 shows "validState (delete e1 R I)"
 proof -
   have A1: "\<forall> (a, b) \<in> folderset I. a \<noteq> e1 \<longrightarrow> (a, b) \<in> folderset (delete e1 R I)"
-  using O1pre
-  unfolding delete_def remove_def delete_pre_def remove_pre_def
-  by auto
+    using O1pre
+    unfolding delete_def remove_def delete_pre_def remove_pre_def
+    by auto
 
   have "\<forall> (a, _) \<in> folderset (delete e1 R I). a \<noteq> e1"
-  using O1pre
-  unfolding delete_def remove_def delete_pre_def remove_pre_def
-  by auto
+    using O1pre
+    unfolding delete_def remove_def delete_pre_def remove_pre_def
+    by auto
 
-  hence "(\<forall> (a, _) \<in> folderset (delete e1 R I) . (filesystem (delete e1 R I)) a \<noteq> None)" using validS
-  unfolding validState_def delete_def remove_def delete_pre_def remove_pre_def
-  by fastforce
+  hence "(\<forall> (a, _) \<in> folderset (delete e1 R I) . (filesystem (delete e1 R I)) a \<noteq> None)" 
+    using validS
+    unfolding validState_def delete_def remove_def delete_pre_def remove_pre_def
+    by fastforce
 
   thus ?thesis
-  using validS A1
-  unfolding validState_def delete_pre_def delete_def remove_def remove_pre_def
-  apply simp
-  by blast
+    using validS A1
+    unfolding validState_def delete_pre_def delete_def remove_def remove_pre_def
+    by (simp, blast)
 qed
-
 
 lemma append_valid:
 fixes
@@ -275,18 +270,17 @@ assumes
 shows "validState (append f1 m1 I)"
 proof -
   have "folderset (append f1 m1 I) = folderset I"
-  unfolding append_def
-  by auto
+    unfolding append_def
+    by auto
 
   hence "(\<forall>f. filesystem (append f1 m1 I) f \<noteq> None \<longrightarrow> (\<exists> (a, _) \<in>folderset (append f1 m1 I). a = f))"
-  using O1pre
-  by (metis (no_types, lifting) append_pre_def append_filesystem case_prod_beta' validS validState_def)
+    using O1pre
+    by (metis (no_types, lifting) append_pre_def append_filesystem case_prod_beta' validS validState_def)
 
   thus ?thesis
-  using O1pre validS
-  unfolding validState_def append_def
-  apply simp
-  by (smt case_prodE fun_upd_apply old.prod.case option.case_eq_if)
+    using O1pre validS
+    unfolding validState_def append_def
+    by (simp add: option.case_eq_if, auto)
 qed
 
 
@@ -302,11 +296,10 @@ assumes
 shows "validState (store f msgold msgnew I)"
 proof -
   show ?thesis
-  using O1pre validS
-  unfolding store_def store_pre_def msgLookup_def Msg_def
-  by (simp add: case_prod_beta' fun_upd_same option.case_eq_if validState_def)
+    using O1pre validS
+    unfolding store_def store_pre_def msgLookup_def msgReplace_def
+    by (simp add: case_prod_beta' fun_upd_same option.case_eq_if validState_def)
 qed
-
 
 lemma expunge_valid:
 fixes
@@ -314,14 +307,14 @@ fixes
   f :: "'a" and
   m :: "'b"
 assumes
-  O1pre: "EXPUNGE_atSource f m I" and
+  O1pre: "expunge_pre f m I" and
   validS: "validState I"
-shows "validState (EXPUNGE_downstream f m I)"
+shows "validState (expunge f m I)"
 proof -
   show ?thesis
-  using O1pre validS
-  unfolding EXPUNGE_atSource_def EXPUNGE_downstream_def msgLookup_def validState_def
-  by (simp add: case_prod_beta' option.case_eq_if)
+    using O1pre validS
+    unfolding expunge_pre_def expunge_def msgLookup_def validState_def
+    by (simp add: case_prod_beta' option.case_eq_if)
 qed
 
 -- "###############################################"
@@ -339,8 +332,6 @@ qed
 -- "  STORE    4      8    11     13     14   "
 -- "                                          "
 -- "EXPUNGE    5      9    12     14     15   "
-
-
 
 -- "Case 1"
 lemma comm_create_create:
@@ -383,28 +374,6 @@ proof -
     by fastforce
   thus ?thesis using A1 by (simp add: delete_def)
 qed
-
--- "Case 6"
-lemma comm_delete_delete:
-fixes
-  I :: "('a, 'b) imap" and
-  R1 :: "'a orset" and
-  R2 :: "'a orset" and
-  f1 :: "'a" and
-  f2 :: "'a"
-assumes
-  O1pre: "delete_pre f1 R1 I" and
-  O2pre: "delete_pre f2 R2 I"
-shows "delete f2 R2 (delete f1 R1 I) = delete f1 R1 (delete f2 R2 I)"
-proof -
-  have A1: "folderset(delete f2 R2 (delete f1 R1 I)) = folderset(delete f1 R1 (delete f2 R2 I))"
-    using O1pre O2pre orset_comm[of "Remove f1 R1" "folderset I" "Remove f2 R2"]
-    by (simp add: delete_pre_def delete_def)
-  have "filesystem(delete f2 R2 (delete f1 R1 I)) = filesystem(delete f1 R1 (delete f2 R2 I))"
-    using O1pre O2pre
-    by (metis (mono_tags, lifting) delete_def fun_upd_twist snd_conv)    
-  thus ?thesis using A1 by (simp add: delete_def)
-qed
   
 -- "Case 3"
 -- "TODO: remove smt"
@@ -425,51 +394,6 @@ proof -
     unfolding append_pre_def append_def create_pre_def create_def lookup_def apply simp
     by (smt case_prodE eq_snd_iff fun_upd_twist option.case_eq_if)
   thus ?thesis by (simp add: append_def create_def)
-qed
-  
--- "Case 7"
-lemma comm_delete_append:
-fixes
-  I :: "('a, 'b) imap" and
-  f1 :: "'a" and
-  f2 :: "'a" and
-  m :: "'b" and
-  R :: "'a orset"
-assumes
-  O1pre: "append_pre f1 m I" and
-  O2pre: "delete_pre f2 R I"
-shows "append f1 m (delete f2 R I) = delete f2 R (append f1 m I)"
-proof -
-  have A1: "folderset(append f1 m (delete f2 R I)) = folderset(delete f2 R (append f1 m I))"
-    by (simp add: append_folderset delete_def)
-  have "filesystem(append f1 m (delete f2 R I)) = filesystem(delete f2 R (append f1 m I))"
-    using O1pre O2pre
-    unfolding append_pre_def append_def delete_pre_def delete_def
-    by (simp add: fun_upd_twist option.case_eq_if)
-  thus ?thesis using A1 prod_eqI  by blast
-qed
-  
--- "Case 10"
--- "TODO: remove smt"
-lemma comm_append_append:
-fixes
-  I :: "('a, 'b) imap" and
-  f1 :: "'a" and
-  f2 :: "'a" and
-  m1 :: "'b" and
-  m2 :: "'b"
-assumes
-  O1pre: "append_pre f1 m1 I" and
-  O2pre: "append_pre f2 m2 I"
-shows "append f1 m1 (append f2 m2 I) = append f2 m2 (append f1 m1 I)"
-proof -
-  have A1: "folderset(append f1 m1 (append f2 m2 I)) = folderset(append f2 m2 (append f1 m1 I))"
-    by (simp add: append_def)
-  have "filesystem(append f1 m1 (append f2 m2 I)) = filesystem(append f2 m2 (append f1 m1 I))"
-    using O1pre O2pre
-    unfolding append_def append_pre_def msgLookup_def
-    by (smt Un_insert_right fun_upd_twist fun_upd_upd insert_commute map_upd_Some_unfold option.case_eq_if option.collapse option.simps(3) snd_conv sup_bot.right_neutral)
-  thus ?thesis using A1 by (simp add: prod_eq_iff)
 qed
   
 -- "Case 4"
@@ -495,6 +419,76 @@ proof -
   thus ?thesis by (simp add: A1 prod.expand)
 qed
   
+-- "Case 5"
+lemma comm_create_expunge:
+fixes
+  I :: "('a, 'b) imap" and
+  f1 :: "'a" and
+  f2 :: "'a" and
+  m :: "'b" and
+  n :: nat
+assumes
+  O1pre: " expunge_pre f1 m I" and
+  O2pre: " create_pre f2 n I"
+shows "expunge f1 m (create f2 n I) = create f2 n (expunge f1 m I)"
+proof -
+  have A1: "folderset (expunge f1 m (create f2 n I)) = folderset (create f2 n (expunge f1 m I))"
+    by (simp add: create_def expunge_def)
+
+  have "filesystem (expunge f1 m (create f2 n I)) = filesystem (create f2 n (expunge f1 m I))"
+    using O1pre O2pre
+    unfolding expunge_pre_def expunge_def create_pre_def create_def
+    by (simp add: fun_upd_twist option.case_eq_if)
+
+  thus ?thesis
+    using A1 prod_eqI
+    by blast
+qed
+  
+-- "Case 6"
+lemma comm_delete_delete:
+fixes
+  I :: "('a, 'b) imap" and
+  R1 :: "'a orset" and
+  R2 :: "'a orset" and
+  f1 :: "'a" and
+  f2 :: "'a"
+assumes
+  O1pre: "delete_pre f1 R1 I" and
+  O2pre: "delete_pre f2 R2 I"
+shows "delete f2 R2 (delete f1 R1 I) = delete f1 R1 (delete f2 R2 I)"
+proof -
+  have A1: "folderset(delete f2 R2 (delete f1 R1 I)) = folderset(delete f1 R1 (delete f2 R2 I))"
+    using O1pre O2pre orset_comm[of "Remove f1 R1" "folderset I" "Remove f2 R2"]
+    by (simp add: delete_pre_def delete_def)
+  have "filesystem(delete f2 R2 (delete f1 R1 I)) = filesystem(delete f1 R1 (delete f2 R2 I))"
+    using O1pre O2pre
+    by (metis (mono_tags, lifting) delete_def fun_upd_twist snd_conv)    
+  thus ?thesis using A1 by (simp add: delete_def)
+qed
+  
+-- "Case 7"
+lemma comm_delete_append:
+fixes
+  I :: "('a, 'b) imap" and
+  f1 :: "'a" and
+  f2 :: "'a" and
+  m :: "'b" and
+  R :: "'a orset"
+assumes
+  O1pre: "append_pre f1 m I" and
+  O2pre: "delete_pre f2 R I"
+shows "append f1 m (delete f2 R I) = delete f2 R (append f1 m I)"
+proof -
+  have A1: "folderset(append f1 m (delete f2 R I)) = folderset(delete f2 R (append f1 m I))"
+    by (simp add: append_folderset delete_def)
+  have "filesystem(append f1 m (delete f2 R I)) = filesystem(delete f2 R (append f1 m I))"
+    using O1pre O2pre
+    unfolding append_pre_def append_def delete_pre_def delete_def
+    by (simp add: fun_upd_twist option.case_eq_if)
+  thus ?thesis using A1 prod_eqI  by blast
+qed
+  
 -- "Case 8"
 lemma comm_delete_store:
 fixes
@@ -518,6 +512,56 @@ proof -
   thus ?thesis by (simp add: A1 prod.expand)
 qed
   
+-- "Case 9"
+lemma comm_delete_expunge:
+fixes
+  I :: "('a, 'b) imap" and
+  f1 :: "'a" and
+  f2 :: "'a" and
+  m :: "'b" and
+  R :: "'a orset"
+assumes
+  O1pre: " expunge_pre f1 m I" and
+  O2pre: " delete_pre f2 R I"
+shows "expunge f1 m (delete f2 R I) = delete f2 R (expunge f1 m I)"
+proof -
+  have A1: "folderset(expunge f1 m (delete f2 R I)) = folderset (delete f2 R (expunge f1 m I))"
+    unfolding delete_def expunge_def
+    by simp
+
+  have "filesystem(expunge f1 m (delete f2 R I)) = filesystem (delete f2 R (expunge f1 m I))"
+    using O1pre O2pre
+    unfolding expunge_pre_def expunge_def delete_pre_def delete_def msgLookup_def
+    by (simp add: fun_upd_twist option.case_eq_if)
+
+  thus ?thesis
+    using A1 prod_eqI
+    by blast
+qed
+  
+-- "Case 10"
+-- "TODO: remove smt"
+lemma comm_append_append:
+fixes
+  I :: "('a, 'b) imap" and
+  f1 :: "'a" and
+  f2 :: "'a" and
+  m1 :: "'b" and
+  m2 :: "'b"
+assumes
+  O1pre: "append_pre f1 m1 I" and
+  O2pre: "append_pre f2 m2 I"
+shows "append f1 m1 (append f2 m2 I) = append f2 m2 (append f1 m1 I)"
+proof -
+  have A1: "folderset(append f1 m1 (append f2 m2 I)) = folderset(append f2 m2 (append f1 m1 I))"
+    by (simp add: append_def)
+  have "filesystem(append f1 m1 (append f2 m2 I)) = filesystem(append f2 m2 (append f1 m1 I))"
+    using O1pre O2pre
+    unfolding append_def append_pre_def msgLookup_def
+    by (smt Un_insert_right fun_upd_twist fun_upd_upd insert_commute map_upd_Some_unfold option.case_eq_if option.collapse option.simps(3) snd_conv sup_bot.right_neutral)
+  thus ?thesis using A1 by (simp add: prod_eq_iff)
+qed
+  
 -- "Case 11"
 lemma comm_append_store:
 fixes
@@ -535,10 +579,37 @@ proof -
   have A1: "folderset (store f1 mo mn (append f2 m I)) = folderset (append f2 m (store f1 mo mn I))"
     by (simp add: append_def store_folderset)
   have "filesystem (store f1 mo mn (append f2 m I)) = filesystem(append f2 m (store f1 mo mn I))"
-    using O1pre O2pre unfolding store_def append_def append_pre_def store_pre_def Msg_def msgLookup_def
+    using O1pre O2pre unfolding store_def append_def append_pre_def store_pre_def msgReplace_def msgLookup_def
     apply (simp add: case_prod_beta') 
     by (smt Diff_empty Diff_insert0 Un_Diff Un_insert_left Un_insert_right fun_upd_twist fun_upd_upd insert_Diff insert_Diff1 map_upd_Some_unfold option.case_eq_if option.collapse option.simps(3) singletonI snd_conv)
   thus ?thesis using A1 by (simp add: prod.expand)
+qed
+  
+-- "Case 12"
+lemma comm_append_expunge:
+fixes
+  I :: "('a, 'b) imap" and
+  f1 :: "'a" and
+  f2 :: "'a" and
+  m1 :: "'b" and
+  m2 :: "'b"
+assumes
+  O1pre: "expunge_pre f1 m1 I" and
+  O2pre: "append_pre f2 m2 I"
+shows "expunge f1 m1 (append f2 m2 I) = append f2 m2 (expunge f1 m1 I)"
+proof -
+  have A1: "folderset (expunge f1 m1 (append f2 m2 I)) = folderset (append f2 m2 (expunge f1 m1 I))"
+    unfolding expunge_def append_def
+    by simp
+
+  have "filesystem (expunge f1 m1 (append f2 m2 I)) = filesystem (append f2 m2 (expunge f1 m1 I))"
+    using O1pre O2pre
+    unfolding expunge_def expunge_pre_def append_def append_pre_def
+    by (smt Diff_empty Diff_insert0 Un_Diff case_prod_beta' fun_upd_apply fun_upd_twist fun_upd_upd insert_Diff insert_Diff1 map_upd_eqD1 mk_disjoint_insert msgLookup_def option.case_eq_if option.collapse option.simps(3) singletonI snd_conv)
+
+  thus ?thesis
+    using A1 prod_eqI
+    by blast
 qed
 
 -- "Case 13"
@@ -590,11 +661,11 @@ proof -
       by blast
     have "x = (S - {mo2}) \<union> {mn2}"
       using Ass Ass2 Ass3
-      unfolding store_def Msg_def
+      unfolding store_def msgReplace_def
       by simp
     hence Ass6: "y = (S - {mo1,mo2}) \<union> {mn1,mn2}"
       using Ass Ass2 Ass3 Ass4 O1pre O2pre
-      unfolding store_def Msg_def store_pre_def
+      unfolding store_def msgReplace_def store_pre_def
       by auto
     have "\<exists> w . filesystem (store f1 mo1 mn1 I) f1 = Some w"
       using Ass
@@ -603,7 +674,7 @@ proof -
       by blast
     hence Ass9: "w = (S - {mo1}) \<union> {mn1}"
       using Ass Ass2
-      unfolding store_def Msg_def
+      unfolding store_def msgReplace_def
       by simp
     have "filesystem(store f2 mo2 mn2 (store f1 mo1 mn1 I)) f1 \<noteq> None"
       using O1pre Ass Ass2
@@ -615,7 +686,7 @@ proof -
       by blast
     hence "z = (S - {mo1,mo2}) \<union> {mn1,mn2}"
       using Ass Ass2 Ass9 Ass8 O1pre O2pre
-      unfolding store_def Msg_def store_pre_def
+      unfolding store_def msgReplace_def store_pre_def
       by auto
     thus "filesystem (store f2 mo1 mn1 (store f2 mo2 mn2 I)) f2 = filesystem (store f2 mo2 mn2 (store f2 mo1 mn1 I)) f2"
       using Ass7 Ass4 Ass6 Ass
@@ -623,27 +694,103 @@ proof -
   qed
 
   thus ?thesis
-  using A1 A2
-  by (smt O1pre O2pre store_def fun_upd_same fun_upd_twist fun_upd_upd option.case_eq_if prod_eqI snd_conv store_not_none)
+    using A1 A2
+    by (smt O1pre O2pre store_def fun_upd_same fun_upd_twist fun_upd_upd option.case_eq_if prod_eqI snd_conv store_not_none)
 qed
+
+-- "Case 14"
+lemma comm_store_expunge:
+fixes
+  I :: "('a, 'b) imap" and
+  f1 :: "'a" and
+  f2 :: "'a" and
+  m :: "'b" and
+  mo :: "'b" and
+  mn :: "'b"
+assumes
+  O1pre: "expunge_pre f1 m1 I" and
+  O2pre: "store_pre f2 mo mn I"
+shows "expunge f1 m1 (store f2 mo mn I) = store f2 mo mn (expunge f1 m1 I)"
+proof -
+  have A1: "folderset (expunge f1 m1 (store f2 mo mn I)) = folderset (store f2 mo mn (expunge f1 m1 I))"
+    by (simp add: expunge_def store_def)
+
+  have A2: "\<forall> f . f1 \<noteq> f2 \<longrightarrow> filesystem (expunge f1 m1 (store f2 mo mn I)) f = filesystem (store f2 mo mn (expunge f1 m1 I)) f"
+    using O1pre O2pre
+    unfolding expunge_def expunge_pre_def store_def store_pre_def
+    by (smt fun_upd_other fun_upd_twist option.case_eq_if snd_conv)
+
+  have A3: "\<forall> f . (f1 = f2 \<and> f \<noteq> f1) \<longrightarrow> filesystem (expunge f1 m1 (store f2 mo mn I)) f = filesystem (store f2 mo mn (expunge f1 m1 I)) f"
+    using O1pre O2pre
+    unfolding expunge_def expunge_pre_def store_def store_pre_def
+    by (smt fun_upd_other fun_upd_twist option.case_eq_if snd_conv)
+
+  have "f1 = f2 \<longrightarrow> filesystem (expunge f1 m1 (store f2 mo mn I)) f1 = filesystem (store f2 mo mn (expunge f1 m1 I)) f1"
+    using O1pre O2pre
+    unfolding expunge_def expunge_pre_def store_def store_pre_def msgLookup_def msgReplace_def
+    by (smt Diff_empty Diff_insert Diff_insert0 Un_Diff empty_iff fun_upd_same insertE insert_commute map_upd_eqD1 option.case_eq_if option.collapse option.simps(3) snd_conv)
+
+  hence "filesystem (expunge f1 m1 (store f2 mo mn I)) = filesystem (store f2 mo mn (expunge f1 m1 I))"
+    using O1pre O2pre A2 A3
+    unfolding expunge_def expunge_pre_def store_def store_pre_def
+    by fastforce
+
+  thus ?thesis
+    using A1 prod_eqI
+    by blast
+qed
+
+-- "Case 15"
+lemma comm_expunge_expunge:
+fixes
+  I :: "('a, 'b) imap" and
+  f1 :: "'a" and
+  f2 :: "'a" and
+  m1 :: "'b" and
+  m2 :: "'b"
+assumes
+  O1pre: " expunge_pre f1 m1 I" and
+  O2pre: " expunge_pre f2 m2 I"
+shows "expunge f1 m1 (expunge f2 m2 I) = expunge f2 m2 (expunge f1 m1 I)"
+proof -
+  have A1: "folderset (expunge f1 m1 (expunge f2 m2 I)) = folderset (expunge f2 m2 (expunge f1 m1 I))"
+    unfolding expunge_def expunge_pre_def
+    by simp
+
+  have "filesystem (expunge f1 m1 (expunge f2 m2 I)) = filesystem (expunge f2 m2 (expunge f1 m1 I))"
+    using O1pre O2pre
+    unfolding expunge_def expunge_pre_def msgLookup_def
+    by (smt Diff_insert fun_upd_twist fun_upd_upd insert_commute map_upd_Some_unfold option.case_eq_if option.collapse option.simps(3) snd_conv)
+
+  thus ?thesis
+  using A1
+  by (simp add: prod_eqI)
+qed
+  
 -- "###############################################"
 -- "### Framework ###"
 -- "###############################################"  
 
-datatype ('a, 'b) ops = Create 'a nat | Delete 'a "'a orset" | Append 'a 'b | Store 'a 'b 'b
+datatype ('a, 'b) ops = 
+  Create 'a nat | 
+  Delete 'a "'a orset" | 
+  Append 'a 'b | 
+  Store 'a 'b 'b |
+  Expunge 'a 'b
 
 fun imap_downstream :: "('a, 'b) ops \<Rightarrow> ('a, 'b) imap \<Rightarrow> ('a,'b) imap" where
   "imap_downstream (Create f n) imap = create f n imap"
 | "imap_downstream (Delete f R) imap = delete f R imap"
 | "imap_downstream (Append f m) imap = append f m imap"
 | "imap_downstream (Store f mo mn) imap = store f mo mn imap"
-  
+| "imap_downstream (Expunge f m) imap = expunge f m imap"  
   
 fun imap_atSource :: "('a, 'b) ops \<Rightarrow> ('a, 'b) imap \<Rightarrow> bool" where
   "imap_atSource (Create f n) imap = create_pre f n imap"
 | "imap_atSource (Delete f R) imap = delete_pre f R imap"
 | "imap_atSource (Append f m) imap = append_pre f m imap"
 | "imap_atSource (Store f mo mn) imap = store_pre f mo mn imap"
+| "imap_atSource (Expunge f m) imap = expunge_pre f m imap"
   
 theorem imap_comm :
 fixes
@@ -670,6 +817,9 @@ proof (cases O1)
     next
       case (Store f2 mo mn)
       then show ?thesis using C1 comm_create_store O1pre O2pre by simp
+    next
+      case (Expunge f2 m)
+      then show ?thesis using C1 comm_create_expunge O1pre O2pre by simp
     qed
 next
   case (Delete f1 R1)
@@ -687,6 +837,9 @@ next
     next
       case (Store f2 mo mn)
       then show ?thesis using C2 comm_delete_store O1pre O2pre by simp
+    next
+      case (Expunge f2 m)
+      then show ?thesis using C2 comm_delete_expunge O1pre O2pre by simp
     qed
 next
   case (Append f1 m1)
@@ -704,6 +857,9 @@ next
     next
       case (Store f2 mo mn)
       then show ?thesis using C3 comm_append_store O1pre O2pre by simp
+    next
+      case (Expunge f2 m)
+      then show ?thesis using C3 comm_append_expunge O1pre O2pre by simp
     qed
 next
   case (Store f1 mo1 mn1)
@@ -721,165 +877,30 @@ next
     next
       case (Store f2 mo mn)
       then show ?thesis using C4 comm_store_store O1pre O2pre by simp
+    next
+      case (Expunge f2 m)
+      then show ?thesis using C4 comm_store_expunge O1pre O2pre by simp
+    qed
+next
+  case (Expunge f1 m1)
+  assume C5: "O1 = Expunge f1 m1"
+  then show ?thesis
+    proof (cases O2)
+      case (Create f2 n)
+      then show ?thesis using C5 comm_create_expunge[of f1 m1 I f2 n] O1pre O2pre by simp
+    next
+      case (Delete f2 R)
+      then show ?thesis using C5 comm_delete_expunge[of f1 m1 I f2 R] O1pre O2pre by simp
+    next
+      case (Append f2 m2)
+      then show ?thesis using C5 comm_append_expunge[of f1 m1 I f2 m2] O1pre O2pre by simp
+    next
+      case (Store f2 mo mn)
+      then show ?thesis using C5 comm_store_expunge[of f1 m1 I f2 mo mn] O1pre O2pre by simp
+    next
+      case (Expunge f2 m)
+      then show ?thesis using C5 comm_expunge_expunge O1pre O2pre by simp
     qed
 qed
-  
--- "###############################################"
--- "### TODO ###"
--- "###############################################"
-
--- "Case 5"
-lemma commCREATE_EXPUNGE:
-fixes
-  I :: "('a, 'b) imap" and
-  f1 :: "'a" and
-  f2 :: "'a" and
-  m :: "'b" and
-  n :: nat
-assumes
-  O1pre: " EXPUNGE_atSource f1 m I" and
-  O2pre: " create_pre f2 n I"
-shows "EXPUNGE_downstream f1 m (create f2 n I) = create f2 n (EXPUNGE_downstream f1 m I)"
-proof -
-  have A1: "folderset (EXPUNGE_downstream f1 m (create f2 n I)) = folderset (create f2 n (EXPUNGE_downstream f1 m I))"
-  unfolding create_def EXPUNGE_downstream_def
-  by simp
-
-  have "filesystem (EXPUNGE_downstream f1 m (create f2 n I)) = filesystem (create f2 n (EXPUNGE_downstream f1 m I))"
-  using O1pre O2pre
-  unfolding EXPUNGE_atSource_def EXPUNGE_downstream_def create_pre_def create_def
-  by (simp add: fun_upd_twist option.case_eq_if)
-
-  thus ?thesis
-  using A1 prod_eqI
-  by blast
-qed
-  
--- "Case 9"
-lemma commDELETE_EXPUNGE:
-fixes
-  I :: "('a, 'b) imap" and
-  f1 :: "'a" and
-  f2 :: "'a" and
-  m :: "'b" and
-  R :: "'a orset"
-assumes
-  O1pre: " EXPUNGE_atSource f1 m I" and
-  O2pre: " delete_pre f2 R I"
-shows "EXPUNGE_downstream f1 m (delete f2 R I) = delete f2 R (EXPUNGE_downstream f1 m I)"
-proof -
-  have A1: "folderset(EXPUNGE_downstream f1 m (delete f2 R I)) = folderset (delete f2 R (EXPUNGE_downstream f1 m I))"
-  unfolding delete_def EXPUNGE_downstream_def
-  by simp
-
-  have "filesystem(EXPUNGE_downstream f1 m (delete f2 R I)) = filesystem (delete f2 R (EXPUNGE_downstream f1 m I))"
-  using O1pre O2pre
-  unfolding EXPUNGE_atSource_def EXPUNGE_downstream_def delete_pre_def delete_def msgLookup_def
-  by (simp add: fun_upd_twist option.case_eq_if)
-
-  thus ?thesis
-  using A1 prod_eqI
-  by blast
-qed
-
--- "Case 12"
-lemma commAPPEND_EXPUNGE:
-fixes
-  I :: "('a, 'b) imap" and
-  f1 :: "'a" and
-  f2 :: "'a" and
-  m1 :: "'b" and
-  m2 :: "'b"
-assumes
-  O1pre: "EXPUNGE_atSource f1 m1 I" and
-  O2pre: "append_pre f2 m2 I"
-shows "EXPUNGE_downstream f1 m1 (append f2 m2 I) = append f2 m2 (EXPUNGE_downstream f1 m1 I)"
-proof -
-  have A1: "folderset (EXPUNGE_downstream f1 m1 (append f2 m2 I)) = folderset (append f2 m2 (EXPUNGE_downstream f1 m1 I))"
-  unfolding EXPUNGE_downstream_def append_def
-  by simp
-
-  have "filesystem (EXPUNGE_downstream f1 m1 (append f2 m2 I)) = filesystem (append f2 m2 (EXPUNGE_downstream f1 m1 I))"
-  using O1pre O2pre
-  unfolding EXPUNGE_downstream_def EXPUNGE_atSource_def append_def append_pre_def
-  by (smt Diff_empty Diff_insert0 Un_Diff case_prod_beta' fun_upd_apply fun_upd_twist fun_upd_upd insert_Diff insert_Diff1 map_upd_eqD1 mk_disjoint_insert msgLookup_def option.case_eq_if option.collapse option.simps(3) singletonI snd_conv)
-
-  thus ?thesis
-  using A1 prod_eqI
-  by blast
-qed
-
--- "Case 14"
-lemma commSTORE_EXPUNGE:
-fixes
-  I :: "('a, 'b) imap" and
-  f1 :: "'a" and
-  f2 :: "'a" and
-  m :: "'b" and
-  mo :: "'b" and
-  mn :: "'b"
-assumes
-  O1pre: "EXPUNGE_atSource f1 m1 I" and
-  O2pre: "store_pre f2 mo mn I"
-shows "EXPUNGE_downstream f1 m1 (store f2 mo mn I) = store f2 mo mn (EXPUNGE_downstream f1 m1 I)"
-proof -
-  have A1: "folderset (EXPUNGE_downstream f1 m1 (store f2 mo mn I)) = folderset (store f2 mo mn (EXPUNGE_downstream f1 m1 I))"
-  unfolding EXPUNGE_downstream_def store_def
-  by simp
-
-  have A2: "\<forall> f . f1 \<noteq> f2 \<longrightarrow> filesystem (EXPUNGE_downstream f1 m1 (store f2 mo mn I)) f = filesystem (store f2 mo mn (EXPUNGE_downstream f1 m1 I)) f"
-  using O1pre O2pre
-  unfolding EXPUNGE_downstream_def EXPUNGE_atSource_def store_def store_pre_def
-  by (smt fun_upd_other fun_upd_twist option.case_eq_if snd_conv)
-
-  have A3: "\<forall> f . (f1 = f2 \<and> f \<noteq> f1) \<longrightarrow> filesystem (EXPUNGE_downstream f1 m1 (store f2 mo mn I)) f = filesystem (store f2 mo mn (EXPUNGE_downstream f1 m1 I)) f"
-  using O1pre O2pre
-  unfolding EXPUNGE_downstream_def EXPUNGE_atSource_def store_def store_pre_def
-  by (smt fun_upd_other fun_upd_twist option.case_eq_if snd_conv)
-
-  have "f1 = f2 \<longrightarrow> filesystem (EXPUNGE_downstream f1 m1 (store f2 mo mn I)) f1 = filesystem (store f2 mo mn (EXPUNGE_downstream f1 m1 I)) f1"
-  using O1pre O2pre
-  unfolding EXPUNGE_downstream_def EXPUNGE_atSource_def store_def store_pre_def msgLookup_def Msg_def
-  by (smt Diff_empty Diff_insert Diff_insert0 Un_Diff empty_iff fun_upd_same insertE insert_commute map_upd_eqD1 option.case_eq_if option.collapse option.simps(3) snd_conv)
-
-  hence "filesystem (EXPUNGE_downstream f1 m1 (store f2 mo mn I)) = filesystem (store f2 mo mn (EXPUNGE_downstream f1 m1 I))"
-  using O1pre O2pre A2 A3
-  unfolding EXPUNGE_downstream_def EXPUNGE_atSource_def store_def store_pre_def
-  by fastforce
-
-  thus ?thesis
-  using A1 prod_eqI
-  by blast
-qed
-
-
--- "Case 15"
-lemma commEXPUNGE_EXPUNGE:
-fixes
-  I :: "('a, 'b) imap" and
-  f1 :: "'a" and
-  f2 :: "'a" and
-  m1 :: "'b" and
-  m2 :: "'b"
-assumes
-  O1pre: " EXPUNGE_atSource f1 m1 I" and
-  O2pre: " EXPUNGE_atSource f2 m2 I"
-shows "EXPUNGE_downstream f1 m1 (EXPUNGE_downstream f2 m2 I) = EXPUNGE_downstream f2 m2 (EXPUNGE_downstream f1 m1 I)"
-proof -
-  have A1: "folderset (EXPUNGE_downstream f1 m1 (EXPUNGE_downstream f2 m2 I)) = folderset (EXPUNGE_downstream f2 m2 (EXPUNGE_downstream f1 m1 I))"
-  unfolding EXPUNGE_downstream_def EXPUNGE_atSource_def
-  by simp
-
-  have "filesystem (EXPUNGE_downstream f1 m1 (EXPUNGE_downstream f2 m2 I)) = filesystem (EXPUNGE_downstream f2 m2 (EXPUNGE_downstream f1 m1 I))"
-  using O1pre O2pre
-  unfolding EXPUNGE_downstream_def EXPUNGE_atSource_def msgLookup_def
-  by (smt Diff_insert fun_upd_twist fun_upd_upd insert_commute map_upd_Some_unfold option.case_eq_if option.collapse option.simps(3) snd_conv)
-
-  thus ?thesis
-  using A1
-  by (simp add: prod_eqI)
-qed
-
-
 
 end
