Isabelle/ORSet.thy
@@ -64,37 +64,34 @@ fixes
 assumes
   O1pre: "orset_atSource O1 S" and
   O2pre: "orset_atSource O2 S"
-shows "orset_downstream O2 (orset_downstream O1 S) = orset_downstream O1 (orset_downstream O2 S)"    
-proof (cases O1)  
+shows "orset_downstream O2 (orset_downstream O1 S) = orset_downstream O1 (orset_downstream O2 S)"
+proof (cases O1)
   case (Add e1 n1)
   assume C1: "O1 = Add e1 n1"
   then show ?thesis 
     proof (cases O2)
       case (Add e2 n2)
       then show ?thesis
-      using C1 O1pre O2pre
-      by (simp add: Un_commute add_def)
+        using C1 O1pre O2pre
+        by (simp add: Un_commute add_def)
     next
-      case (Remove e2 R)
+      case (Remove e2 R) 
       then show ?thesis
-      using C1 O1pre O2pre
-      apply (simp add: add_pre_def add_def remove_pre_def remove_def) 
-      by auto
+        using C1 O1pre O2pre
+        by (simp add: add_pre_def add_def remove_pre_def remove_def, auto)
     qed
 next
   case (Remove e1 R1)
   assume C2: "O1 = Remove e1 R1"
   then show ?thesis 
     proof (cases O2)
-      case (Add e2 n)
+      case (Add e2 n) 
       then show ?thesis using C2 O1pre O2pre
-      apply (simp add: add_pre_def add_def remove_pre_def remove_def)
-      by auto        
+        by (simp add: add_pre_def add_def remove_pre_def remove_def, auto)      
     next
       case (Remove e2 R)
       then show ?thesis using C2 O1pre O2pre
-      apply (simp add: remove_def remove_pre_def) 
-      by auto
+        by (simp add: remove_def remove_pre_def, auto)
     qed
 qed
 
